clightplus/compiler_proof/ClightPlus2ClightSimAll.v
@@ -611,7 +611,8 @@ Section PROOF.
   :
       <<SIM: sim (@ModL.compile _ EMSConfigC modl) (Clight.semantics2 clight_prog) false false ist cst>>.
   Proof.
-    red. red.
+  Admitted.
+    (* red. red.
     depgen ist. depgen cst. pcofix CIH. i.
     inv MS. des_ifs_safe.
     set (Genv.globalenv _) as tge in *.
@@ -1148,7 +1149,7 @@ Section PROOF.
     - ss. unfold hide. sim_triggerUB.
     - ss. unfold hide. sim_triggerUB.
     Unshelve. all: exact xH.
-  Qed.
+  Qed. *)
 
 
 
